\documentclass[11pt, a4paper]{article}
\usepackage{a4wide}
\usepackage{amsmath, amsfonts, dsfont, booktabs, graphicx, natbib, a4, times, microtype, hyperref}
\newcommand{\E}{\ensuremath{{\mathbb E}}} % expected value
\def\func#1{\mathop{\rm #1}}
\begin{document}
\title{Solution to Exercise 5}
\author{Simon A.\ Broda}
\date{}
\maketitle

\begin{enumerate}


\item See Jupyter notebook.
\item
\begin{enumerate}
\item Splitting out the first term of the sum immediately yields
\begin{align*}
 \widehat{\sigma}_{t+1,EWMA}^{2}  &=(1-\lambda )\sum_{j=0}^{\infty }\lambda ^{j}r_{t-j}^{2} \\
 \widehat{\sigma}_{t+1,EWMA}^{2}  &=(1-\lambda ) \lambda^0 r_{t-0}^2+(1-\lambda )\sum_{j=1}^{\infty }\lambda ^{j}r_{t-j}^{2} \\
 \widehat{\sigma}_{t+1,EWMA}^{2}  &=(1-\lambda ) r_{t}^2+(1-\lambda )\sum_{j=0}^{\infty }\lambda ^{j+1}r_{t-1-j}^{2} \\
 \widehat{\sigma}_{t+1,EWMA}^{2}  &=(1-\lambda ) r_{t}^2+\lambda(1-\lambda )\sum_{j=0}^{\infty }\lambda ^{j}r_{t-1-j}^{2} \\
&=(1-\lambda )r_{t}^{2}+\lambda\widehat{\sigma}_{t,EWMA}^{2}.
\end{align*}
%\item Solving $\widehat{\sigma}^2=\hat{\omega} /(1-\hat\alpha -\hat\beta )$ for $\hat{\omega}$, we find $\hat{\omega}=\widehat{\sigma}^2\cdot(1-\hat\alpha -\hat\beta )$. Plugging this into
%the equation
%\begin{align*}
%\widehat{\sigma} _{t+1}^{2}&=\hat{\omega}+\hat{\alpha}\hat{u}_{t}^{2}+\hat{\beta} \widehat{\sigma} _{t}^{2}\\
%\intertext{yields}
%\widehat{\sigma} _{t+1}^{2}&=\widehat{\sigma}^2\cdot(1-\hat\alpha -\hat\beta )+\hat{\alpha}\hat{u}_{t}^{2}+\hat{\beta} \widehat{\sigma} _{t}^{2}\\
%&=\widehat{\sigma}^2+\hat{\alpha}(\hat{u}_{t}^{2}-\widehat{\sigma}^2)+\hat{\beta} (\widehat{\sigma} _{t}^{2}-\widehat{\sigma}^2).
%\end{align*}
%\item
%The result of the previous question also implies that
%\begin{align}
%\widehat{\sigma} _{t+2}^{2}&=\widehat{\sigma}^2+\hat{\alpha}(\hat{u}_{t+1}^{2}-\widehat{\sigma}^2)+\hat{\beta} (\widehat{\sigma} _{t+1}^{2}-\widehat{\sigma}^2).\notag
%\intertext{Replacing the unknown $\hat{u}_{t+1}^{2}$ with its forecast $\widehat{\sigma} _{t+1}^{2}$, we see that}
%\widehat{\sigma} _{t+2}^{2}&=\widehat{\sigma}^2+\hat{\alpha}(\widehat{\sigma} _{t+1}^{2}-\widehat{\sigma}^2)+\hat{\beta} (\widehat{\sigma} _{t+1}^{2}-\widehat{\sigma}^2)\notag\\
%\widehat{\sigma} _{t+2}^{2}&=\widehat{\sigma} ^{2}+(\hat\alpha+\hat\beta) (\widehat{\sigma}_{t+1}^{2}-\widehat{\sigma} ^{2}).\label{eq1}\\
%\intertext{Equation \eqref{eq1} also implies that}
%\widehat{\sigma} _{t+3}^{2}&=\widehat{\sigma} ^{2}+(\hat\alpha+\hat\beta) (\widehat{\sigma}_{t+2}^{2}-\widehat{\sigma} ^{2}),\label{eq2}\\
%\intertext{and plugging \eqref{eq1} into \eqref{eq2} results in}
%\widehat{\sigma} _{t+3}^{2}&=\widehat{\sigma} ^{2}+(\hat\alpha+\hat\beta) ((\hat\alpha+\hat\beta) (\widehat{\sigma}_{t+1}^{2}-\widehat{\sigma} ^{2}))\notag\\
%&=\widehat{\sigma} ^{2}+(\hat\alpha+\hat\beta)^2 (\widehat{\sigma}_{t+1}^{2}-\widehat{\sigma} ^{2}).\notag\\
%\intertext{Iterating this process produces}
%\widehat{\sigma} _{t+s}^{2}&=\widehat{\sigma} ^{2}+(\hat\alpha+\hat\beta)^{s-1} (\widehat{\sigma}_{t+1}^{2}-\widehat{\sigma} ^{2})\notag
%\end{align}
%as claimed.

\end{enumerate}
\end{enumerate}
\end{document} 